verification/tests/TestMutString.fst
@@ -1,0 +1,11 @@
+module TestMutString
+open FStar.String
+open FStar.Char
+
+let rec f (fuel:int) : Tot (int * (list char)) (decreases fuel) =
+  if fuel <= 0 then (0, [])
+  else (1, ['a'])
+
+and g (fuel:int) : Tot (string * (list char)) (decreases fuel) =
+  if fuel <= 0 then ("", [])
+  else ("hi", ['b'])
