verification/tests/TestOL.fst
@@ -1,0 +1,16 @@
+module TestOL
+open FStar.List.Tot
+open FStar.Char
+open FStar.String
+
+let rec f (fuel:int) (cs:list char) (acc:int) : Tot (int * (list char)) (decreases fuel) =
+  if fuel <= 0 then (acc, cs)
+  else match cs with
+  | c :: rest -> f (fuel - 1) rest acc
+  | [] -> (acc, cs)
+
+and g (fuel:int) (cs:list char) (acc:list char) : Tot (string * (list char)) (decreases fuel) =
+  if fuel <= 0 then ("", cs)
+  else match cs with
+  | c :: rest -> g (fuel - 1) rest (c :: acc)
+  | [] -> ("", [])
