verification/tests/TestTrace.fst
@@ -1,0 +1,82 @@
+module TestTrace
+open FStar.List.Tot
+open FStar.Pervasives
+open FStar.Char
+module U32 = FStar.UInt32
+
+type tok =
+  | TkL
+  | TkR
+  | TkN of int
+  | TkS of string
+
+type expr =
+  | Num of int
+  | Add of (expr * expr)
+
+val is_ws : char -> bool
+let is_ws c = c = ' ' || c = '
+' || c = '	'
+
+val is_digit : char -> bool
+let is_digit c =
+  let n = U32.v (u32_of_char c) in
+  n >= U32.v (u32_of_char '0') && n <= U32.v (u32_of_char '9')
+
+val is_sym : char -> bool
+let is_sym c = not (is_ws c) && c <> '(' && c <> ')'
+
+val dv : char -> int
+let dv c = U32.v (u32_of_char c) - U32.v (u32_of_char '0')
+
+let rec do_tok (fuel:int) (cs:list char) : Tot (list tok) (decreases fuel) =
+  if fuel <= 0 then []
+  else match cs with
+  | [] -> []
+  | c :: rest ->
+    if is_ws c then do_tok (fuel - 1) rest
+    else if c = '(' then TkL :: do_tok (fuel - 1) rest
+    else if c = ')' then TkR :: do_tok (fuel - 1) rest
+    else if is_digit c then
+      let (n, r) = do_pn (fuel - 1) cs 0 in
+      TkN n :: do_tok (fuel - 1) r
+    else do_tok (fuel - 1) rest
+
+and do_pn (fuel:int) (cs:list char) (acc:int) : Tot (int * (list char)) (decreases fuel) =
+  if fuel <= 0 then (acc, cs)
+  else match cs with
+  | c :: rest ->
+    if is_digit c then do_pn (fuel - 1) rest (Prims.op_Multiply acc 10 + dv c)
+    else (acc, cs)
+  | [] -> (acc, [])
+
+let rec do_par (fuel:int) (toks:list tok) : Tot (option expr) (decreases fuel) =
+  if fuel <= 0 then None
+  else match toks with
+  | [] -> None
+  | TkN n :: [] -> Some (Num n)
+  | TkL :: TkS "+" :: TkN a :: TkN b :: TkR :: [] -> Some (Add (Num a, Num b))
+  | _ -> None
+
+let rec do_ev (fuel:int) (e:expr) : Tot int (decreases fuel) =
+  if fuel <= 0 then 0
+  else match e with
+  | Num n -> n
+  | Add (a, b) -> do_ev (fuel - 1) a + do_ev (fuel - 1) b
+
+val run : string -> Tot int
+let run s =
+  let cs = FStar.String.list_of_string s in
+  let toks = do_tok 100 cs in
+  match do_par 100 toks with
+  | Some e -> do_ev 20 e
+  | None -> 0
+
+val t1 : unit -> Lemma (run "42" = 42)
+let t1 () = assert_norm (run "42" = 42)
+
+val t2 : unit -> Lemma (run "(+ 3 4)" = 7)
+let t2 () = assert_norm (run "(+ 3 4)" = 7)
+
+val t3 : unit -> Lemma (run "42" = 999)
+let t3 () = assert_norm (run "42" = 999)
