verification/tests/TestTupleType.fst
@@ -1,0 +1,7 @@
+module TestTupleType
+
+type p = int * int
+
+let f () : Tot p = (1, 2)
+
+let g () : Tot (int * int) = (1, 2)
